+hoare example

ClassicalLanguage/de_hoare.lean
@@ -6,7 +6,7 @@ import ClassicalLanguage.de_BSOS
 def hoare(P: Cond)(prog: Program)(Q: Cond): Prop :=
     ∀sStart sFin: State, evalC P sStart → BSOS sStart prog sFin → evalC Q sFin
 
-lemma strengthPostCond (Qn: Cond)(P Q: Cond)(prog: Program):
+lemma strnegthPostCond (Q: Cond)(Qn: Cond)(P: Cond)(prog: Program):
     fol Q Qn → hoare P prog Q → hoare P prog Qn := by
   intro stronger
   intro hoare1
@@ -22,7 +22,7 @@ lemma strengthPostCond (Qn: Cond)(P Q: Cond)(prog: Program):
   apply stronger sFin
   apply postCond
 
-lemma weakenPreCond (Pn: Cond)(P Q: Cond)(prog: Program):
+lemma weakenPreCond (P: Cond)(Pn: Cond)(Q: Cond)(prog: Program):
     fol Pn P → hoare P prog Q → hoare Pn prog Q := by
     intro weaker
     intro hoare1
@@ -117,3 +117,66 @@ theorem hoareWhile(Q: Cond)(cond: Cond)(body: Program):
     simp
     clear preCond hoareBody body Q
     aesop
+
+-- Example
+
+def increm(name: String): Program := Program.assign name (Expr.sum (Expr.var name) (Expr.num 1))
+
+def decision(name: String): Cond := Cond.less (Expr.var name) (Expr.num 50)
+
+def less100(name: String): Cond := Cond.less (Expr.var name) (Expr.num 100)
+
+def cycle: Program :=
+Program.whilee (less100 "i")
+               (Program.seq
+                          (increm "i")
+                          (Program.iff
+                                      (decision "i")
+                                      (increm "j")
+                                      Program.skip
+                          )
+
+               )
+
+def invar:Cond := Cond.less (Expr.var "j") (Expr.var "i")
+
+theorem example1: hoare invar cycle invar := by
+  apply strnegthPostCond (Cond.and invar (Cond.not (less100 "i")))
+  {
+    rw [fol]
+    intro s
+    rw [evalC]
+    aesop
+  }
+  apply hoareWhile
+  let condInter:Cond := Cond.less (Expr.sum (Expr.var "j") (Expr.num 1)) (Expr.var "i")
+  apply hoareSeq invar condInter invar
+  {
+    have eq: fol invar (replC condInter "i" (Expr.sum (Expr.var "i") (Expr.num 1))) := by
+      simp [replC, condInter, Expr.var, invar, replE, evalC, evalE, fol]
+    apply weakenPreCond (replC condInter "i" (Expr.sum (Expr.var "i") (Expr.num 1)))
+    apply eq
+    apply hoareAssign "i" (Expr.sum (Expr.var "i") (Expr.num 1)) condInter
+  }
+  {
+    apply hoareIf
+    {
+      apply weakenPreCond (replC invar "j" (Expr.sum (Expr.var "j") (Expr.num 1)))
+      simp [fol, evalC, replC, condInter, evalE, invar, replE]
+      apply hoareAssign
+    }
+    {
+      apply weakenPreCond invar
+      simp [replC, condInter, Expr.var, invar, replE, evalC, evalE, fol, State]
+      clear condInter
+      {
+        intro s
+        intro neq
+        apply @Int.lt_trans (s "j") (s "j" + 1) (s "i")
+        apply Int.lt_add_of_pos_right
+        simp
+        apply neq
+      }
+      apply hoareSkip
+    }
+  }
